Clean up interp file

theories/Core/Utils.v
@@ -11,7 +11,7 @@ Ltac next := unfold bt; cbn.
 Tactic Notation "cbn*" := next.
 
 Polymorphic Class MonadTrigger (E : Type -> Type) (M : Type -> Type) : Type :=
-  mtrigger : E ~> M.
+  mtrigger : forall {X}, E X -> M X.
 
 Polymorphic Class MonadBr (B : Type -> Type) (M : Type -> Type) : Type :=
   mbr : forall (b : bool) {X} (b: B X), M X.
