theories/Interp/Interp.v
@@ -18,11 +18,81 @@ Import CTreeNotations.
 Open Scope ctree_scope.
 
 (* end hide *)
-Definition translateF {E F C R} (h : E ~> F) (rec: ctree E C R -> ctree F C R) (t : ctreeF E C R _) : ctree F C R  :=
+
+(** ** Fold *)
+
+(** The most general shape of fold over the structure takes two parameters:
+    - an event handler [E ~> M] describing how to implement events
+    - a local scheduler [B ~> M] describing valid branches
+    and defines for it a monad morphism [ctree E B ~> M]
+    for any monad [M] with a loop operator. *)
+Definition fold {E B M : Type -> Type}
+  {FM : Functor M} {MM : Monad M} {IM : MonadIter M}
+  (h : E ~> M) (g : bool -> B ~> M) :
+	ctree E B ~> M :=
+  fun R =>
+		iter (fun t =>
+				    match observe t with
+				    | RetF r => ret (inr r)
+				    | BrF b c k => fmap (fun x => inl (k x)) (g b _ c)
+				    | VisF e k => fmap (fun x => inl (k x)) (h _ e)
+				    end).
+
+Arguments fold {E B M FM MM IM} h g [T].
+
+(** Unfolding of [fold]. *)
+Notation fold_ h g t :=
+  (match observe t with
+  | RetF r => Ret r
+	| VisF e k => bind (h _ e) (fun x => Guard (fold h g (k x)))
+	| BrF b c k => bind (g b _ c) (fun x => Guard (fold h g (k x)))
+  end)%function.
+
+(** Implementing simultaneously external events while refining
+    the internal non-determinism is somewhat uncommon.
+    We hence also define two particular case:
+    - [interp] only implements external events, and re-emit branches
+    without cutting them (internalized in [M] via [MonadBr]
+    - [refine] only refines the internal branches,
+    and re-emit external events (internalized in [M] via [MonadTrigger]
+  *)
+
+Definition interp {E B M : Type -> Type}
+  {FM : Functor M} {MM : Monad M} {IM : MonadIter M} {BM : MonadBr B M}
+  (h : E ~> M) := fold h (fun b _ c => mbr b c).
+
+Arguments interp {E B M FM MM IM BM} h [T].
+
+(** Unfolding of [interp]. *)
+Notation interp_ h t :=
+  (match observe t with
+  | RetF r => Ret r
+	| VisF e k => bind (h _ e) (fun x => Guard (interp h (k x)))
+	| BrF b c k => bind (mbr b c) (fun x => Guard (interp h (k x)))
+  end)%function.
+
+Definition refine {E B M : Type -> Type}
+  {FM : Functor M} {MM : Monad M} {IM : MonadIter M} {TM : MonadTrigger E M}
+  (g : bool -> B ~> M) := fold (fun _ e => mtrigger e) g.
+
+Arguments refine {E B M FM MM IM TM} g [T].
+
+(** Unfolding of [refine]. *)
+Notation refine_ g t :=
+  (match observe t with
+  | RetF r => Ret r
+	| VisF e k => bind (mtrigger e) (fun x => Guard (refine g (k x)))
+	| BrF b c k => bind (g b _ c) (fun x => Guard (refine g (k x)))
+  end)%function.
+
+Definition translateF {E F C R}
+  (h : E ~> F)
+  (rec: ctree E C R -> ctree F C R)
+  (t : ctreeF E C R _) : ctree F C R  :=
 	match t with
-		| RetF x => Ret x
-		| VisF e k => Vis (h _ e) (fun x => rec (k x))
-		| BrF b c k => Br b c (fun x => rec (k x))
+	| RetF x => Ret x
+	| VisF e k => Vis (h _ e) (fun x => rec (k x))
+	| BrF b c k => Br b c (fun x => rec (k x))
 	end.
 
 Definition translate {E F C} (h : E ~> F) : ctree E C ~> ctree F C
@@ -30,34 +100,8 @@ Definition translate {E F C} (h : E ~> F) : ctree E C ~> ctree F C
 
 Arguments translate {E F C} h [T].
 
-(** ** Interpret *)
 
-(** An event handler [E ~> M] defines a monad morphism
-		[ctree E C ~> M] for any monad [M] with a loop operator. *)
-Definition interp {E C M : Type -> Type}
-           {FM : Functor M} {MM : Monad M} {IM : MonadIter M}
-           (h : E ~> M) (h' : bool -> C ~> M) :
-			ctree E C ~> M := fun R =>
-			iter (fun t =>
-				match observe t with
-				| RetF r => ret (inr r)
-				| BrF b c k => fmap (fun x => inl (k x)) (h' b _ c)
-				| VisF e k => fmap (fun x => inl (k x)) (h _ e)
-				end).
-
-Arguments interp {E C M FM MM IM} h h' [T].
-
-(** Unfolding of [interp]. *)
-Notation interp_ h h' t :=
-  (match observe t with
-  | RetF r => Ret r
-	| VisF e k => bind (h _ e) (fun x => Guard (interp h h' (k x)))
-	| BrF b c k => bind (h' b _ c) (fun x => Guard (interp h h' (k x)))
-  end)%function.
-
-Notation interpE h := (interp h (fun b _ c => branch b c)).
-
-(* TODO [step] should refold  *)
+(* TODO MOVE *)
 Lemma bind_br {E C R S X} b (c : C X) (k : _ -> ctree E C R) (h : _ -> ctree E C S):
       (Br b c k) >>= h ≅ Br b c (fun x => k x >>= h).
 Proof.
@@ -65,96 +109,198 @@ Proof.
   reflexivity.
 Qed.
 
-Section Interp.
+(** Establishing generic results on [fold] is tricky: because it goes into
+    a very generic monad [M], it requires some heavy axiomatization of this
+    monad. Yoon et al.'s ICFP'22 develop the necessary tools to this end.
+    For now, we simply specialize results to specific [M]s.
+ *)
+Section FoldCTree.
 
-  Context {E F C D: Type -> Type} {X : Type} `{B1 -< D}
-          {h : E ~> ctree F D} {h' : bool -> C ~> ctree F D}.
+  Section With_Params.
 
-  (** ** [interpE] and constructors *)
+    (** Specialization to [M = ctree F D] *)
+    Context {E F C D: Type -> Type} {X : Type} `{B1 -< D}
+      {h : E ~> ctree F D} {g : bool -> C ~> ctree F D}.
 
-  (** These are specializations of [unfold_interpE], which can be added as
-      rewrite hints.
+    (** ** [interpE] and constructors *)
+
+    (** Unfold lemma. *)
+    Lemma unfold_fold (t: ctree E C X):
+      fold h g t ≅ fold_ h g t.
+    Proof.
+      unfold fold, Basics.iter, MonadIter_ctree, mbr, MonadBr_ctree, CTree.branch.
+      rewrite unfold_iter.
+      destruct (observe t); cbn.
+      - now rewrite ?bind_ret_l.
+      - now rewrite bind_map, ?bind_ret_l.
+      - now rewrite bind_map.
+    Qed.
+
+    Lemma fold_ret (x: X):
+      fold h g (Ret x) ≅ Ret x.
+    Proof. now rewrite unfold_fold. Qed.
+
+    Lemma fold_vis {U} (e: E U) (k: U -> ctree E C X) :
+      fold h g (Vis e k) ≅ x <- h _ e;; Guard (fold h g (k x)).
+    Proof. now rewrite unfold_fold. Qed.
+
+    Lemma fold_br {U} b (c : C U) (k: _ -> ctree E C X) :
+      fold h g (Br b c k) ≅ x <- g b _ c;; Guard (fold h g (k x)).
+    Proof. now rewrite unfold_fold. Qed.
+
+    #[global] Instance fold_equ :
+      Proper (equ eq ==> equ eq) (fold h g (T := X)).
+    Proof.
+      cbn.
+      coinduction ? CIH.
+      intros * EQ; step in EQ.
+      rewrite 2 unfold_fold.
+      inv EQ; auto.
+      - cbn -[ebt].
+        upto_bind_eq.
+        constructor; intros ?; auto.
+      - cbn -[ebt].
+        upto_bind_eq.
+        constructor; intros ?; auto.
+    Qed.
+
+    (** Unfold lemma. *)
+    Lemma unfold_interp `{C -< D} (t: ctree E C X):
+      interp h t ≅ interp_ h t.
+    Proof.
+      unfold interp,fold, Basics.iter, MonadIter_ctree, mbr, MonadBr_ctree, CTree.branch.
+      rewrite unfold_iter.
+      destruct (observe t); cbn.
+      - now rewrite ?bind_ret_l.
+      - now rewrite bind_map, ?bind_ret_l.
+      - now rewrite bind_map.
+    Qed.
+
+    Lemma interp_ret `{C -< D} (x: X):
+      interp h (Ret x : ctree E C X) ≅ Ret x.
+    Proof. now rewrite unfold_interp. Qed.
+
+    Lemma interp_vis `{C -< D} {U} (e: E U) (k: U -> ctree E C X) :
+      interp h (Vis e k) ≅ x <- h _ e;; Guard (interp h (k x)).
+    Proof. now rewrite unfold_interp. Qed.
+
+    Lemma interp_br `{C -< D} {U} b (c : C U) (k: _ -> ctree E C X) :
+      interp h (Br b c k) ≅ x <- branch b c;; Guard (interp h (k x)).
+    Proof. now rewrite unfold_interp. Qed.
+
+    #[global] Instance interp_equ `{C -< D} :
+      Proper (equ eq ==> equ eq) (interp (B := C) (M := ctree F D) h (T := X)).
+    Proof.
+      cbn.
+      coinduction ? CIH.
+      intros * EQ; step in EQ.
+      rewrite 2 unfold_interp.
+      inv EQ; auto.
+      - cbn -[ebt].
+        upto_bind_eq.
+        constructor; intros ?; auto.
+      - cbn -[ebt].
+        upto_bind_eq.
+        constructor; intros ?; auto.
+    Qed.
+
+    (** Unfold lemma. *)
+    Lemma unfold_refine `{E -< F} (t: ctree E C X):
+      refine g t ≅ refine_ g t.
+    Proof.
+      unfold refine,fold, Basics.iter, MonadIter_ctree, mbr, MonadBr_ctree, CTree.branch.
+      rewrite unfold_iter.
+      destruct (observe t); cbn.
+      - now rewrite ?bind_ret_l.
+      - now rewrite bind_map, ?bind_ret_l.
+      - now rewrite bind_map.
+    Qed.
+
+    Lemma refine_ret `{E -< F} (x: X):
+      refine g (Ret x : ctree E C X) ≅ Ret x.
+    Proof. now rewrite unfold_refine. Qed.
+
+    Lemma refine_vis `{E -< F} {U} (e: E U) (k: U -> ctree E C X) :
+      refine g (Vis e k) ≅ x <- trigger e;; Guard (refine g (k x)).
+    Proof. now rewrite unfold_refine. Qed.
+
+    Lemma refine_br `{E -< F} {U} b (c : C U) (k: _ -> ctree E C X) :
+      refine g (Br b c k) ≅ x <- g b _ c;; Guard (refine g (k x)).
+    Proof. now rewrite unfold_refine. Qed.
+
+    #[global] Instance refine_equ `{E -< F} :
+      Proper (equ eq ==> equ eq) (refine (E := E) (M := ctree F _) g (T := X)).
+    Proof.
+      cbn.
+      coinduction ? CIH.
+      intros * EQ; step in EQ.
+      rewrite 2 unfold_refine.
+      inv EQ; auto.
+      - cbn -[ebt].
+        upto_bind_eq.
+        constructor; intros ?; auto.
+      - cbn -[ebt].
+        upto_bind_eq.
+        constructor; intros ?; auto.
+    Qed.
+
+  End With_Params.
+
+  (** The following fact specialises further [interp] so that events are implemented into ctrees whose index for branches is unchanged.
+      Most likely, this is the case in all applications.
    *)
-
-  (** Unfold lemma. *)
-  Lemma unfold_interp (t: ctree E C X):
-    interp h h' t ≅ interp_ h h' t.
+  Lemma interp_guard {E F C X} `{B1 -< C} (h' : E ~> ctree F C) (t: ctree E C X):
+    interp h' (Guard t) ≅ Guard (Guard (interp h' t)).
   Proof.
-    unfold interpE, Basics.iter, MonadIter_ctree, mbr, MonadBr_ctree, CTree.branch.
-    rewrite unfold_iter.
-    destruct (observe t); cbn.
-    - now rewrite ?bind_ret_l.
-    - now rewrite bind_map, ?bind_ret_l.
-    - now rewrite bind_map. 
+    rewrite unfold_interp. setoid_rewrite bind_br.
+    apply equ_BrF. intro.
+    rewrite bind_ret_l. reflexivity.
   Qed.
 
-  Lemma interp_ret (x: X):
-    interp h h' (Ret x) ≅ Ret x.  
-  Proof. now rewrite unfold_interp. Qed.
+  Section InterpBind.
 
-  Lemma interp_vis {U} (e: E U) (k: U -> ctree E C X) :
-    interp h h' (Vis e k) ≅ x <- h _ e;; Guard (interp h h' (k x)).
-  Proof. now rewrite unfold_interp. Qed.
+    Context {E F C D: Type -> Type} {X : Type} `{B1 -< D}.
 
-  Lemma interp_br {U} b (c : C U) (k: _ -> ctree E C X) :
-    interp h h' (Br b c k) ≅ x <- h' b _ c;; Guard (interp h h' (k x)).
-  Proof. now rewrite unfold_interp. Qed.
+    Lemma fold_bind (h : E ~> ctree F D) (g : bool -> C ~> ctree F D) {S} (t : ctree E C X) (k : X -> ctree _ _ S) :
+      fold h g (t >>= k) ≅ fold h g t >>= (fun x => fold h g (k x)).
+    Proof.
+      revert t.
+      coinduction X' CIH.
+      intros t.
+      rewrite unfold_bind, (unfold_fold t).
+      desobs t; cbn -[ebt].
+      - now rewrite bind_ret_l.
+      - rewrite fold_vis, bind_bind.
+        upto_bind_eq.
+        rewrite bind_guard.
+        now constructor.
+      - rewrite fold_br, bind_bind.
+        upto_bind_eq.
+        rewrite bind_guard.
+        now constructor.
+    Qed.
 
-  #[global] Instance interp_equ :
-    Proper (equ eq ==> equ eq) (interp h h' (T := X)).
-  Proof.
-    cbn.
-    coinduction ? CIH.
-    intros * EQ; step in EQ.
-    rewrite 2 unfold_interp.
-    inv EQ; auto.
-    - cbn -[ebt].
-      upto_bind_eq.
-      constructor; intros ?; auto.
-    - cbn -[ebt].
-      upto_bind_eq.
-      constructor; intros ?; auto.
-  Qed.
+    Lemma interp_bind (h : E ~> ctree F D) `{C -< D} {S} (t : ctree E C X) (k : X -> ctree _ _ S) :
+      interp h (t >>= k) ≅ interp h t >>= (fun x => interp h (k x)).
+    Proof.
+      unfold interp.
+      now rewrite fold_bind.
+    Qed.
 
-End Interp.
+    Lemma refine_bind (g : bool -> C ~> ctree F D) `{E -< F} {S} (t : ctree E C X) (k : X -> ctree _ _ S) :
+      refine g (t >>= k) ≅ refine g t >>= (fun x => refine g (k x)).
+    Proof.
+      unfold refine.
+      now rewrite fold_bind.
+    Qed.
 
-Lemma interpE_guard {E F C X} `{B1 -< C} {h : E ~> ctree F C} (t: ctree E C X):
-  interpE h (Guard t) ≅ Guard (Guard (interpE h t)).
-Proof.
-  rewrite unfold_interp. setoid_rewrite bind_br.
-  apply equ_BrF. intro.
-  rewrite bind_ret_l. reflexivity.
-Qed.
+  End InterpBind.
 
-Section InterpBind.
+End FoldCTree.
 
-  Context {E F C D: Type -> Type} {X : Type} `{B1 -< D}.
-  Context {h : E ~> ctree F D} {h' : bool -> C ~> ctree F D}.
-
-  (* Note: this is specialized to [ctree F] as target monad. *)
-  (* TODO: Incorporate Irene's work to generalize *)
-  Lemma interp_bind {S} (t : ctree E C X) (k : X -> ctree _ _ S) :
-    interp h h' (t >>= k) ≅ interp h h' t >>= (fun x => interp h h' (k x)).
-  Proof.
-    revert t.
-    coinduction X' CIH.
-    intros t.
-    rewrite unfold_bind, (unfold_interp t).
-    desobs t; cbn -[ebt].
-    - now rewrite bind_ret_l.
-    - rewrite interp_vis, bind_bind.
-      upto_bind_eq.
-      rewrite bind_guard.
-      now constructor.
-    - rewrite interp_br, bind_bind.
-      upto_bind_eq.
-      rewrite bind_guard.
-      now constructor.
-  Qed.
-
-End InterpBind.
-
-(*| Counter-example showing that interpE does not preserve sbisim in the general case. |*)
+(*|
+Counter-example showing that interpE does not preserve sbisim in the general case.
+|*)
 
 Inductive VoidE : Type -> Type :=
 | voidE : VoidE void.
@@ -176,7 +322,7 @@ Proof.
   intros. destruct H. exact (Step stuckD).
 Defined.
 
-Example interpE_sbsisim_counterexample : ~ (interpE h t1 ~ interpE h t2).
+Example interpE_sbsisim_counterexample : ~ (interp h t1 ~ interp h t2).
 Proof.
   red. intros. unfold t2 in H.
   playR in H.
@@ -186,4 +332,3 @@ Proof.
   apply trans_guard. setoid_rewrite unfold_interp. cbn. rewrite bind_step. etrans.
   rewrite unfold_interp in TR. unfold t1, h in TR. cbn in TR. inv_trans.
 Qed.
-
